Move heap taint field to vale_full_heap record

vale/code/arch/Vale.Arch.Heap.fst
@@ -9,19 +9,27 @@ let heap_impl = vale_full_heap
 
 let heap_get hi = hi.vf_heap.mh
 
-let heap_upd hi mh' =
+let heap_taint hi = hi.vf_taint
+
+let heap_upd hi mh' mt' =
   let h' = mi_heap_upd hi.vf_heap mh' in
   {
     vf_layout = hi.vf_layout;
     vf_heap = h';
     vf_heaplets = Map16.upd hi.vf_heaplets 0 h';
+    vf_taint = mt';
   }
 
 let heap_create_machine ih =
   down_mem ih
 
-let heap_create_impl ih =
+let heap_create_impl ih mt =
   let vh = ValeHeap (down_mem ih) (Ghost.hide ih) in
   let vh4 = ((vh, vh), (vh, vh)) in
   let vh16 = ((vh4, vh4), (vh4, vh4)) in
-  {vf_layout = {vl_old_heap = vh}; vf_heap = vh; vf_heaplets = Map16.upd vh16 0 vh}
+  {
+    vf_layout = {vl_old_heap = vh};
+    vf_heap = vh;
+    vf_heaplets = Map16.upd vh16 0 vh;
+    vf_taint = mt;
+  }
